heap_lang/lifting.v
@@ -1,10 +1,9 @@
-From iris.program_logic Require Export weakestpre.
-From iris.heap_lang Require Export lang.
-From iris.program_logic Require Import lifting.
+From iris.program_logic Require Export ectx_weakestpre.
 From iris.program_logic Require Import ownership. (* for ownP *)
+From iris.heap_lang Require Export lang.
 From iris.heap_lang Require Import tactics.
 Import uPred.
-Local Hint Extern 0 (language.reducible _ _) => do_step ltac:(eauto 2).
+Local Hint Extern 0 (head_reducible _ _) => do_step eauto 2.
 
 Section lifting.
 Context {Σ : iFunctor}.
@@ -13,10 +12,10 @@ Implicit Types Φ : val → iProp heap_lang Σ.
 Implicit Types K : ectx.
 Implicit Types ef : option (expr []).
 
-(** Bind. *)
+(** Bind. This bundles some arguments that wp_ectx_bind leaves as indices. *)
 Lemma wp_bind {E e} K Φ :
   WP e @ E {{ λ v, WP fill K (of_val v) @ E {{ Φ }} }} ⊢ WP fill K e @ E {{ Φ }}.
-Proof. apply: weakestpre.wp_bind. Qed.
+Proof. exact: wp_ectx_bind. Qed.
 
 (** Base axioms for core primitives of the language: Stateful reductions. *)
 Lemma wp_alloc_pst E σ e v Φ :
@@ -27,7 +26,7 @@ Proof.
   (* TODO: This works around ssreflect bug #22. *)
   intros. set (φ (e' : expr []) σ' ef := ∃ l,
     ef = None ∧ e' = Loc l ∧ σ' = <[l:=v]>σ ∧ σ !! l = None).
-  rewrite -(wp_lift_atomic_step (Alloc e) φ σ) // /φ;
+  rewrite -(wp_lift_atomic_head_step (Alloc e) φ σ) // /φ;
     last (by intros; inv_step; eauto 8); last (by simpl; eauto).
   apply sep_mono, later_mono; first done.
   apply forall_intro=>v2; apply forall_intro=>σ2; apply forall_intro=>ef.
@@ -43,7 +42,7 @@ Lemma wp_load_pst E σ l v Φ :
   σ !! l = Some v →
   (▷ ownP σ ★ ▷ (ownP σ -★ Φ v)) ⊢ WP Load (Loc l) @ E {{ Φ }}.
 Proof.
-  intros. rewrite -(wp_lift_atomic_det_step σ v σ None) ?right_id //;
+  intros. rewrite -(wp_lift_atomic_det_head_step σ v σ None) ?right_id //;
     last (by intros; inv_step; eauto using to_of_val); simpl; by eauto.
 Qed.
 
@@ -52,7 +51,7 @@ Lemma wp_store_pst E σ l e v v' Φ :
   (▷ ownP σ ★ ▷ (ownP (<[l:=v]>σ) -★ Φ (LitV LitUnit)))
   ⊢ WP Store (Loc l) e @ E {{ Φ }}.
 Proof.
-  intros. rewrite -(wp_lift_atomic_det_step σ (LitV LitUnit) (<[l:=v]>σ) None)
+  intros. rewrite-(wp_lift_atomic_det_head_step σ (LitV LitUnit) (<[l:=v]>σ) None)
     ?right_id //; last (by intros; inv_step; eauto); simpl; by eauto.
 Qed.
 
@@ -61,7 +60,7 @@ Lemma wp_cas_fail_pst E σ l e1 v1 e2 v2 v' Φ :
   (▷ ownP σ ★ ▷ (ownP σ -★ Φ (LitV $ LitBool false)))
   ⊢ WP CAS (Loc l) e1 e2 @ E {{ Φ }}.
 Proof.
-  intros. rewrite -(wp_lift_atomic_det_step σ (LitV $ LitBool false) σ None)
+  intros. rewrite -(wp_lift_atomic_det_head_step σ (LitV $ LitBool false) σ None)
     ?right_id //; last (by intros; inv_step; eauto);
     simpl; split_and?; by eauto.
 Qed.
@@ -71,7 +70,7 @@ Lemma wp_cas_suc_pst E σ l e1 v1 e2 v2 Φ :
   (▷ ownP σ ★ ▷ (ownP (<[l:=v2]>σ) -★ Φ (LitV $ LitBool true)))
   ⊢ WP CAS (Loc l) e1 e2 @ E {{ Φ }}.
 Proof.
-  intros. rewrite -(wp_lift_atomic_det_step σ (LitV $ LitBool true)
+  intros. rewrite -(wp_lift_atomic_det_head_step σ (LitV $ LitBool true)
     (<[l:=v2]>σ) None) ?right_id //; last (by intros; inv_step; eauto);
     simpl; split_and?; by eauto.
 Qed.
@@ -80,7 +79,7 @@ Qed.
 Lemma wp_fork E e Φ :
   (▷ Φ (LitV LitUnit) ★ ▷ WP e {{ λ _, True }}) ⊢ WP Fork e @ E {{ Φ }}.
 Proof.
-  rewrite -(wp_lift_pure_det_step (Fork e) (Lit LitUnit) (Some e)) //=;
+  rewrite -(wp_lift_pure_det_head_step (Fork e) (Lit LitUnit) (Some e)) //=;
     last by intros; inv_step; eauto.
   rewrite later_sep -(wp_value _ _ (Lit _)) //.
 Qed.
@@ -90,7 +89,7 @@ Lemma wp_rec E f x e1 e2 v Φ :
   ▷ WP subst' x e2 (subst' f (Rec f x e1) e1) @ E {{ Φ }}
   ⊢ WP App (Rec f x e1) e2 @ E {{ Φ }}.
 Proof.
-  intros. rewrite -(wp_lift_pure_det_step (App _ _)
+  intros. rewrite -(wp_lift_pure_det_head_step (App _ _)
     (subst' x e2 (subst' f (Rec f x e1) e1)) None) //= ?right_id;
     intros; inv_step; eauto.
 Qed.
@@ -106,7 +105,7 @@ Lemma wp_un_op E op l l' Φ :
   un_op_eval op l = Some l' →
   ▷ Φ (LitV l') ⊢ WP UnOp op (Lit l) @ E {{ Φ }}.
 Proof.
-  intros. rewrite -(wp_lift_pure_det_step (UnOp op _) (Lit l') None)
+  intros. rewrite -(wp_lift_pure_det_head_step (UnOp op _) (Lit l') None)
     ?right_id -?wp_value //; intros; inv_step; eauto.
 Qed.
 
@@ -114,21 +113,21 @@ Lemma wp_bin_op E op l1 l2 l' Φ :
   bin_op_eval op l1 l2 = Some l' →
   ▷ Φ (LitV l') ⊢ WP BinOp op (Lit l1) (Lit l2) @ E {{ Φ }}.
 Proof.
-  intros Heval. rewrite -(wp_lift_pure_det_step (BinOp op _ _) (Lit l') None)
+  intros Heval. rewrite -(wp_lift_pure_det_head_step (BinOp op _ _) (Lit l') None)
     ?right_id -?wp_value //; intros; inv_step; eauto.
 Qed.
 
 Lemma wp_if_true E e1 e2 Φ :
   ▷ WP e1 @ E {{ Φ }} ⊢ WP If (Lit (LitBool true)) e1 e2 @ E {{ Φ }}.
 Proof.
-  rewrite -(wp_lift_pure_det_step (If _ _ _) e1 None)
+  rewrite -(wp_lift_pure_det_head_step (If _ _ _) e1 None)
     ?right_id //; intros; inv_step; eauto.
 Qed.
 
 Lemma wp_if_false E e1 e2 Φ :
   ▷ WP e2 @ E {{ Φ }} ⊢ WP If (Lit (LitBool false)) e1 e2 @ E {{ Φ }}.
 Proof.
-  rewrite -(wp_lift_pure_det_step (If _ _ _) e2 None)
+  rewrite -(wp_lift_pure_det_head_step (If _ _ _) e2 None)
     ?right_id //; intros; inv_step; eauto.
 Qed.
 
@@ -136,7 +135,7 @@ Lemma wp_fst E e1 v1 e2 v2 Φ :
   to_val e1 = Some v1 → to_val e2 = Some v2 →
   ▷ Φ v1 ⊢ WP Fst (Pair e1 e2) @ E {{ Φ }}.
 Proof.
-  intros. rewrite -(wp_lift_pure_det_step (Fst _) e1 None)
+  intros. rewrite -(wp_lift_pure_det_head_step (Fst _) e1 None)
     ?right_id -?wp_value //; intros; inv_step; eauto.
 Qed.
 
@@ -144,7 +143,7 @@ Lemma wp_snd E e1 v1 e2 v2 Φ :
   to_val e1 = Some v1 → to_val e2 = Some v2 →
   ▷ Φ v2 ⊢ WP Snd (Pair e1 e2) @ E {{ Φ }}.
 Proof.
-  intros. rewrite -(wp_lift_pure_det_step (Snd _) e2 None)
+  intros. rewrite -(wp_lift_pure_det_head_step (Snd _) e2 None)
     ?right_id -?wp_value //; intros; inv_step; eauto.
 Qed.
 
@@ -152,7 +151,7 @@ Lemma wp_case_inl E e0 v0 e1 e2 Φ :
   to_val e0 = Some v0 →
   ▷ WP App e1 e0 @ E {{ Φ }} ⊢ WP Case (InjL e0) e1 e2 @ E {{ Φ }}.
 Proof.
-  intros. rewrite -(wp_lift_pure_det_step (Case _ _ _)
+  intros. rewrite -(wp_lift_pure_det_head_step (Case _ _ _)
     (App e1 e0) None) ?right_id //; intros; inv_step; eauto.
 Qed.
 
@@ -160,7 +159,7 @@ Lemma wp_case_inr E e0 v0 e1 e2 Φ :
   to_val e0 = Some v0 →
   ▷ WP App e2 e0 @ E {{ Φ }} ⊢ WP Case (InjR e0) e1 e2 @ E {{ Φ }}.
 Proof.
-  intros. rewrite -(wp_lift_pure_det_step (Case _ _ _)
+  intros. rewrite -(wp_lift_pure_det_head_step (Case _ _ _)
     (App e2 e0) None) ?right_id //; intros; inv_step; eauto.
 Qed.
 
